Defined tiling transformation for accesses, values, typdefctx, stacks and states.

TrTiling.v
@@ -11,174 +11,187 @@ License: MIT.
 Set Implicit Arguments.
 Require Export Semantics LibSet LibMap TLCbuffer.
 
-(** In order to make this transformation work, we will need to first:
-    - Annotate val_array with the array type.
-    - Annotate array_access with the array type.
-*)
-
-
 (* ********************************************************************** *)
 (* * Definition of the transformation *)
 
-(** Grouping transformation. Specified by:
-    - The name of the struct to be modified.
-    - The set of fields to be grouped.
-    - The name of the new struct that will hold the fields to be grouped.
-    - The name of the field in the new struct that will have as type
-      the new struct. *)
+(** Tiling transformation. Specified by:
+    - The typvar of the array to be tiled.
+    - The new typvar of the tiles.
+    - The size of the tiles. *)
 
-Record group_tr := make_group_tr {
-  group_tr_struct_name : typvar;
-  group_tr_fields : set field;
-  group_tr_new_struct_name : typvar;
-  group_tr_new_struct_field : field
-}. 
+Record tiling_tr := make_tiling_tr {
+  tiling_tr_array_name : typvar;
+  tiling_tr_tile_name : typvar;
+  tiling_tr_tile_size : size
+}.
 
-Notation make_group_tr' := make_group_tr.
+Notation make_tiling_tr' := make_tiling_tr.
+
+(** Checking if the transformation is acceptable *)
+
+Inductive tiling_tr_ok : tiling_tr -> typdefctx -> Prop :=
+  | tiling_tr_ok_intros : forall Ta Tt n T os tt C,
+      tt = make_tiling_tr Ta Tt n ->
+      Ta \indom C ->
+      C[Ta] = typ_array T os ->
+      Tt \notindom C ->
+      (forall Tv,
+        Tv \indom C ->
+        Tv <> Ta ->
+        ~ free_typvar C Tt C[Tv]) ->
+      tiling_tr_ok tt C.
 
 
+(* ********************************************************************** *)
+(* * The transformation applied to the different constructs. *)
+
+(** Transformation of typdefctxs: C ~ |C| *)
+
+Inductive tr_typdefctx (tt:tiling_tr) : typdefctx -> typdefctx -> Prop :=
+  | tr_typdefctx_intro : forall T Tt Ta k os os' C C',
+      tt = make_tiling_tr Ta Tt k ->
+      dom C' = dom C \u \{Tt} ->
+      C[Ta] = typ_array T os ->
+      C'[Ta] = typ_array (typ_var Tt) os' ->
+      C'[Tt] = typ_array T (Some k) ->
+      (forall Tv,
+        Tv \indom C ->
+        Tv <> Ta ->
+        C'[Tv] = C[Tv]) ->
+      (forall n,
+        os = Some n ->
+        os' = Some (n / k)) ->
+      (os = None ->
+        os' = None) ->
+      tr_typdefctx tt C C'.
 
 (** Transformation of paths: π ~ |π| *)
 
-Inductive tr_accesses (gt:group_tr) : accesses -> accesses -> Prop :=
+Inductive tr_accesses (tt:tiling_tr) : accesses -> accesses -> Prop :=
   | tr_accesses_nil :
-      tr_accesses gt nil nil
-  | tr_accesses_array : forall π π' i, 
-      tr_accesses gt π π' ->
-      tr_accesses gt ((access_array i)::π) ((access_array i)::π')
-  | tr_accesses_field_group : forall π π' f fg Ts Tsg,
-      tr_accesses gt π π' ->
-      Ts = group_tr_struct_name gt ->
-      Tsg = group_tr_new_struct_name gt ->
-      f \in (group_tr_fields gt) ->
-      fg = group_tr_new_struct_field gt ->
-      tr_accesses gt ((access_field Ts f)::π) ((access_field Ts fg)::(access_field Tsg f)::π')
-  | tr_accesses_field_other : forall T Ts π π' f,
-      tr_accesses gt π π' ->
-      Ts = group_tr_struct_name gt ->
-      (T <> Ts \/ f \notin (group_tr_fields gt)) ->
-      tr_accesses gt ((access_field T f)::π) ((access_field T f)::π').
+      tr_accesses tt nil nil
+  | tr_accesses_array_tiling : forall π π' Ta Tt i n a0 a1 a2,
+      tr_accesses tt π π' ->
+      tt = make_tiling_tr Ta Tt n ->
+      a0 = access_array (typ_var Ta) i ->
+      a1 = access_array (typ_var Ta) (i/n) ->
+      a2 = access_array (typ_var Tt) (i mod n) ->
+      tr_accesses tt (a0::π) (a1::a2::π')
+  | tr_accesses_array_other : forall π π' T i,
+      T <> typ_var (tiling_tr_array_name tt) ->
+      tr_accesses tt π π' ->
+      tr_accesses tt ((access_array T i)::π) ((access_array T i)::π')
+  | tr_accesses_field : forall T π π' f,
+      tr_accesses tt π π' ->
+      tr_accesses tt ((access_field T f)::π) ((access_field T f)::π').
 
 (** Transformation of values: v ~ |v| *)
 
-Inductive tr_val (gt:group_tr) : val -> val -> Prop :=
+Inductive tr_val (tt:tiling_tr) : val -> val -> Prop :=
   | tr_val_error :
-      tr_val gt val_error val_error
+      tr_val tt val_error val_error
   | tr_val_uninitialized :
-      tr_val gt val_uninitialized val_uninitialized
+      tr_val tt val_uninitialized val_uninitialized
   | tr_val_unit :
-      tr_val gt val_unit val_unit
+      tr_val tt val_unit val_unit
   | tr_val_bool : forall b,
-      tr_val gt (val_bool b) (val_bool b)
+      tr_val tt (val_bool b) (val_bool b)
   | tr_val_int : forall i,
-      tr_val gt (val_int i) (val_int i)
+      tr_val tt (val_int i) (val_int i)
   | tr_val_double : forall d,
-      tr_val gt (val_double d) (val_double d)
+      tr_val tt (val_double d) (val_double d)
   | tr_val_abstract_ptr : forall l π π',
-      tr_accesses gt π π' ->
-      tr_val gt (val_abstract_ptr l π) (val_abstract_ptr l π')
-  | tr_val_array : forall a a',
+      tr_accesses tt π π' ->
+      tr_val tt (val_abstract_ptr l π) (val_abstract_ptr l π')
+  | tr_val_array_tiling : forall (l:nat) k Tt Ta a a',
+      tt = make_tiling_tr Ta Tt k ->
+      length a = l ->
+      length a' = l / k ->
+      (forall i a'',
+        index a' i ->
+        a'[i] = val_array (typ_var Tt) a'' ->
+        length a'' = k ->
+        (forall j,
+          index a'' j ->
+          tr_val tt a''[j] a''[j])) ->
+      tr_val tt (val_array (typ_var Ta) a) (val_array (typ_var Ta) a')
+  | tr_val_array_other : forall T a a',
+      T <> typ_var (tiling_tr_array_name tt) ->
       length a = length a' ->
       (forall i,
         index a i ->
-        tr_val gt a[i] a'[i]) ->
-      tr_val gt (val_array a) (val_array a')
-  | tr_val_struct_group : forall Ts Tsg s s' fg fs sg,
-      gt = make_group_tr Ts fs Tsg fg ->
-      fs \c dom s ->
-      fg \notindom s ->
-      dom s' = (dom s \- fs) \u \{fg} ->
-      dom sg = fs ->
-      (forall f,
-        f \indom sg ->
-        tr_val gt s[f] sg[f]) ->
-      (forall f,
-        f \notin fs ->
-        f \indom s ->
-        tr_val gt s[f] s'[f]) ->
-      s'[fg] = val_struct Tsg sg ->
-      tr_val gt (val_struct Ts s) (val_struct Ts s')
+        tr_val tt a[i] a'[i]) ->
+      tr_val tt (val_array T a) (val_array T a')
   | tr_val_struct_other : forall T s s',
-      T <> group_tr_struct_name gt ->
       dom s = dom s' ->
       (forall f,
         f \indom s ->
-        tr_val gt s[f] s'[f]) ->
-      tr_val gt (val_struct T s) (val_struct T s').
+        tr_val tt s[f] s'[f]) ->
+      tr_val tt (val_struct T s) (val_struct T s').
 
-Definition is_prim_struct_access (op:prim) :=
+Definition is_array_access (op:prim) :=
   match op with
-  | prim_struct_access _ _ => True
+  | prim_array_access _ => True
+  | prim_array_get _ => True
   | _ => False
   end.
 
 
 (** Transformation of terms: t ~ |t| *)
 
-Inductive tr_trm (gt:group_tr) : trm -> trm -> Prop :=
+Inductive tr_trm (tt:tiling_tr) : trm -> trm -> Prop :=
   | tr_trm_val : forall v v',
-      tr_val gt v v' ->
-      tr_trm gt (trm_val v) (trm_val v')
+      tr_val tt v v' ->
+      tr_trm tt (trm_val v) (trm_val v')
   | tr_trm_var : forall x,
-      tr_trm gt (trm_var x) (trm_var x)
+      tr_trm tt (trm_var x) (trm_var x)
   | tr_trm_if : forall t1 t2 t3 t1' t2' t3',
-      tr_trm gt t1 t1' ->
-      tr_trm gt t2 t2' ->
-      tr_trm gt t3 t3' ->
-      tr_trm gt (trm_if t1 t2 t3) (trm_if t1' t2' t3')
+      tr_trm tt t1 t1' ->
+      tr_trm tt t2 t2' ->
+      tr_trm tt t3 t3' ->
+      tr_trm tt (trm_if t1 t2 t3) (trm_if t1' t2' t3')
   | tr_trm_let : forall x t1 t2 t1' t2',
-      tr_trm gt t1 t1' ->
-      tr_trm gt t2 t2' ->
-      tr_trm gt (trm_let x t1 t2) (trm_let x t1' t2')
+      tr_trm tt t1 t1' ->
+      tr_trm tt t2 t2' ->
+      tr_trm tt (trm_let x t1 t2) (trm_let x t1' t2')
   (* new *)  
   | tr_trm_new : forall T,
-      tr_trm gt (trm_app (prim_new T) nil) (trm_app (prim_new T) nil)
-  (* Special case: struct access *)
-  | tr_trm_struct_access_x : forall p p' s s_g f f_g a1 a2 r,
-      tr_trm gt p p' ->
-      s = group_tr_struct_name gt ->
-      s_g = group_tr_new_struct_name gt ->
-      f \in (group_tr_fields gt) ->
-      f_g = group_tr_new_struct_field gt ->
-      a1 = prim_struct_access s_g f ->
-      a2 = prim_struct_access s f_g ->
-      r = trm_app a1 ((trm_app a2 (p'::nil))::nil) ->
-      tr_trm gt (trm_app (prim_struct_access s f) (p::nil)) r
-  | tr_trm_struct_access_other : forall s p p' T f r,
-      tr_trm gt p p' ->
-      s = group_tr_struct_name gt ->
-      (T <> s \/ f \notin (group_tr_fields gt)) ->
-      r = (trm_app (prim_struct_access T f) (p'::nil)) ->
-      tr_trm gt (trm_app (prim_struct_access T f) (p::nil)) r
+      tr_trm tt (trm_app (prim_new T) nil) (trm_app (prim_new T) nil)
+
+  (* TODO: Special case: array access *)
+  (*
+  | tr_trm_array_access_x :
+  | tr_trm_array_access_other : *)
+
   (* Args *)
   | tr_trm_args1 : forall op t1 t1',
-      ~ is_prim_struct_access op ->
-      tr_trm gt t1 t1' ->
-      tr_trm gt (trm_app op (t1::nil)) (trm_app op (t1'::nil))
+      ~ is_array_access op ->
+      tr_trm tt t1 t1' ->
+      tr_trm tt (trm_app op (t1::nil)) (trm_app op (t1'::nil))
   | tr_trm_args2 : forall op t1 t1' t2 t2',
-      tr_trm gt t1 t1' ->
-      tr_trm gt t2 t2' ->
-      tr_trm gt (trm_app op (t1::t2::nil)) (trm_app op (t1'::t2'::nil)).
+      tr_trm tt t1 t1' ->
+      tr_trm tt t2 t2' ->
+      tr_trm tt (trm_app op (t1::t2::nil)) (trm_app op (t1'::t2'::nil)).
 
 
 (** Transformation of stacks: S ~ |S| *)
 
-Inductive tr_stack_item (gt:group_tr) : (var * val) -> (var * val) -> Prop :=
+Inductive tr_stack_item (tt:tiling_tr) : (var * val) -> (var * val) -> Prop :=
   | tr_stack_item_intro : forall x v v',
-      tr_val gt v v' -> 
-      tr_stack_item gt (x, v) (x, v').
+      tr_val tt v v' -> 
+      tr_stack_item tt (x, v) (x, v').
 
-Inductive tr_stack (gt:group_tr) : stack -> stack -> Prop :=
+Inductive tr_stack (tt:tiling_tr) : stack -> stack -> Prop :=
   | tr_stack_intro : forall S S',
-      LibList.Forall2 (tr_stack_item gt) S S' ->
-      tr_stack gt S S'.
+      LibList.Forall2 (tr_stack_item tt) S S' ->
+      tr_stack tt S S'.
 
-Lemma stack_lookup_tr : forall gt S S' x v,
-  tr_stack gt S S' ->
+Lemma stack_lookup_tr : forall tt S S' x v,
+  tr_stack tt S S' ->
   Ctx.lookup x S = Some v -> 
     exists v', 
        Ctx.lookup x S' = Some v' 
-    /\ tr_val gt v v'.
+    /\ tr_val tt v v'.
 Proof.
   introv HS Hx. inverts HS as HS. induction HS.
   { inverts Hx. }
@@ -191,37 +204,10 @@ Qed.
 
 (** Transformation of states: m ~ |m| *)
 
-Inductive tr_state (gt:group_tr) : state -> state -> Prop :=
+Inductive tr_state (tt:tiling_tr) : state -> state -> Prop :=
   | tr_state_intro : forall m m',
       dom m = dom m' ->
       (forall l,
         l \indom m ->
-        tr_val gt m[l] m'[l]) ->
-      tr_state gt m m'.
-
-
-(** Transformation of typdefctxs: C ~ |C| *)
-
-Inductive tr_typdefctx (gt:group_tr) : typdefctx -> typdefctx -> Prop :=
-  | tr_typdefctx_intro : forall Tt fs Tg fg C C',
-      gt = make_group_tr Tt fs Tg fg ->
-      Tt \indom C ->
-      Tg \notindom C ->
-      dom C' = dom C \u \{Tg} ->
-      (forall T,
-        T \indom C ->
-        T <> Tt ->
-        C'[T] = C[T]) ->
-      fs \c dom (C[Tt]) ->
-      fg \notindom (C[Tt]) ->
-      dom (C'[Tt]) = (dom (C[Tt]) \- fs) \u \{fg} ->
-      (forall f,
-        f \indom (C[Tt]) ->
-        f \notin fs ->
-        C'[Tt][f] = C[Tt][f]) ->
-      C'[Tt][fg] = typ_struct Tg ->
-      dom (C'[Tg]) = fs ->
-      (forall f,
-        f \indom (C'[Tg]) ->
-        C'[Tg][f] = C[Tt][f]) ->
-      tr_typdefctx gt C C'.
+        tr_val tt m[l] m'[l]) ->
+      tr_state tt m m'.
